# â™¾ï¸æé™
## ğŸ’«å¸¸ç”¨ç­‰ä»·æ— ç©·å°
$$
\begin{align}
1- cos^ax = \frac{a}{2}x^2 \\
a^x-1=xlna \\ 
(1+x)^a-1 = ax \\
\end{align}
$$

$$
\begin{align}
(1+x)^{\frac{1}{x} }=e(1-\frac{1}{2}x+\frac{11}{24}x^2  ) \\
ln(x+\sqrt{1+x^2} )=x-\frac{1}{6}x^3 
\end{align}$$


## ğŸ’«å¸¸ç”¨æ³°å‹’å…¬å¼
$$
\begin{align}
\sin x =  x - \frac{1}{6} x^3 \\
\arcsin x = x + \frac{1}{6} x^3
\end{align}
$$

$$
\begin{align}
\tan x = x + \frac{1}{3}x^3 \\
\arctan x = x - \frac{1}{3}x^3
\end{align}
$$


$$
\begin{align}
\cos x = 1 - \frac{1}{2}x^2 + \frac{1}{24}x^4  
\end{align}
$$

$$
\begin{align}
e^x &= 1+x+\frac{1}{2!}x^2+\frac{1}{3!}x^3+\frac{1}{4!}x^4 \\
\ln (1+x)   &=x-\frac{1}{2}x^2 +\frac{1}{3}x^3 \\
\end{align}
$$

$$
\begin{align}
(1+x)^a &= 1+ax+\frac{a(a-1)}{2!}x^2 + \frac{a(a-1)(a-2)}{3!}x^3  \\
\frac{1}{1-x} &= 1+x+x^2+x^3+x^4 \\
\frac{1}{1+x} &= 1-x+x^2-x^3+x^4 
\end{align}
$$

## ğŸ’«0/0å‹
å››ç§è§£æ³•
- ç­‰ä»·æ— ç©·å°
- æ³°å‹’å±•å¼€
- æ´›å¿…è¾¾
- ä¸­å€¼å®šç†

æ´›å¿…è¾¾ä½¿ç”¨åœºæ™¯:
- æ²¡åŠæ³•äº†qaq
- å˜é™ç§¯åˆ†
![[Pasted image 20241007161058.png|400]]
- æŠ½è±¡å‡½æ•°

ä¸­å€¼å®šç†ä½¿ç”¨åœºæ™¯:
- æ‹‰æ ¼æœ—æ—¥: åŒåå‡½æ•°ç›¸å‡
$$
\begin{align}
f(a)-f(b)=f'(\sigma )(a-b)
\end{align}â€‹
$$
![[Pasted image 20241007161322.png|425]]
**æ³¨æ„Ïƒå’Œxçš„å…³ç³»**

- ç§¯åˆ†ä¸­å€¼å®šç†
$$
\begin{align}
\int_{a}^{b} f(x)dx = f(\sigma )(b-a)
\end{align}
$$
![[Pasted image 20241007161545.png|500]]



## ğŸ’«âˆ/âˆ
æ–¹æ³•:
- ç­‰ä»·æ— ç©·å¤§(ä¹˜é™¤æ³•é€‚ç”¨)
- æ´›å¿…è¾¾

$$
\begin{align}
lnx < x^a < e^x
\end{align}
$$

**attention!**
x->0+æ—¶, lnxä¹Ÿå¾ˆæ…¢
x->-âˆæ—¶, e^x ä¹Ÿå¾ˆå¿«

$$
\begin{align}
\lim_{x \to 0^+} xlnx=0 \\
\lim_{x \to -\infty }xe^x=0
\end{align}
$$


## ğŸ’«âˆ-âˆ(éš¾)
*å¤šé¡¹å¼ä¸€èˆ¬åªéœ€è¦ä¿ç•™æ¬¡æ•°æœ€é«˜çš„å‰ä¸¤é¡¹å³å¯*
![[Pasted image 20241007195524.png|400]]


*arctanx*
$$
\begin{align}
\arctan x + \arctan \frac{1}{x} = \frac{\pi }{2}  ,x >0 \\
\arctan x + \arctan \frac{1}{x} = -\frac{\pi }{2}  ,x<0
\end{align}
$$



## ğŸ’«1^âˆ
åŒ–ç®€æˆe^x






